coq/proof/Inject.v
@@ -21,6 +21,11 @@ Require Import SimulationLocal.
 Require InvMem.
 Require InvState.
 
+Set Implicit Arguments.
+
+
+Definition CONF_TODO: Prop. Admitted.
+
 (* TODO: name *)
 Definition inject_locals
            (inv:InvMem.Rel.t)
@@ -37,8 +42,76 @@ Definition inject_allocas
     (fun a_src a_tgt => inv.(InvMem.Rel.inject) a_src = Some (a_tgt, 0))
     alc_src alc_tgt.
 
-Definition CONF_TODO: Prop. Admitted.
+Lemma inject_locals_getOperandValue
+      inv val
+      conf_src locals_src gval_src
+      conf_tgt locals_tgt gval_tgt
+      (CONF: CONF_TODO)
+      (INJECT: inject_locals inv locals_src locals_tgt)
+      (SRC: getOperandValue (CurTargetData conf_src) val locals_src (Globals conf_src) = Some gval_src)
+      (TGT: getOperandValue (CurTargetData conf_tgt) val locals_tgt (Globals conf_tgt) = Some gval_tgt):
+  genericvalues_inject.gv_inject inv.(InvMem.Rel.inject) gval_src gval_tgt.
+Proof.
+  destruct val; ss.
+  - exploit INJECT; eauto. i. des.
+    rewrite TGT in LU_TGT. inv LU_TGT. ss.
+  - admit. (* CONF_TODO *)
+Admitted.
 
+Lemma inject_locals_params2GVs
+      inv0 args0
+      conf_src locals_src gvs_param_src
+      conf_tgt locals_tgt gvs_param_tgt
+      (CONF: CONF_TODO)
+      (INJECT: inject_locals inv0 locals_src locals_tgt)
+      (PARAM_SRC:params2GVs (CurTargetData conf_src) args0 locals_src (Globals conf_src) = Some gvs_param_src)
+      (PARAM_TGT:params2GVs (CurTargetData conf_tgt) args0 locals_tgt (Globals conf_tgt) = Some gvs_param_tgt):
+  list_forall2 (genericvalues_inject.gv_inject (InvMem.Rel.inject inv0)) gvs_param_src gvs_param_tgt.
+Proof.
+  revert gvs_param_src PARAM_SRC.
+  revert gvs_param_tgt PARAM_TGT.
+  induction args0.
+  - i. ss. inv PARAM_SRC. inv PARAM_TGT. econs.
+  - i. ss.
+    destruct a as ((ty_a & attr_a) & v_a).
+    revert PARAM_TGT. revert PARAM_SRC.
+    (* TODO: make a tactic *)
+    repeat
+      (match goal with
+       | [|- context[match ?c with | Some _ => _ | None => _ end]] =>
+         let COND := fresh "COND" in
+         destruct c eqn:COND
+       end; ss).
+    i. inv PARAM_SRC. inv PARAM_TGT.
+    econs.
+    + eapply inject_locals_getOperandValue; eauto.
+    + eauto.
+Qed.
+
+Lemma inject_locals_inj_incr
+      inv0 inv1
+      locals_src locals_tgt
+      (INJECT: inject_locals inv0 locals_src locals_tgt)
+      (INCR: InvMem.Rel.le inv0 inv1):
+  inject_locals inv1 locals_src locals_tgt.
+Proof.
+  ii. exploit INJECT; eauto. i. des.
+  esplits; eauto.
+  eapply genericvalues_inject.gv_inject_incr; try apply INCR; eauto.
+Qed.
+
+Lemma inject_allocas_inj_incr
+      inv0 inv1
+      allocas_src allocas_tgt
+      (INJECT: inject_allocas inv0 allocas_src allocas_tgt)
+      (INCR: InvMem.Rel.le inv0 inv1):
+  inject_allocas inv1 allocas_src allocas_tgt.
+Proof.
+  eapply list_forall2_imply; eauto. s. i.
+  apply INCR. auto.
+Qed.
+
+(* TODO: position *)
 Lemma targetdata_dec
       (TD_src TD_tgt:TargetData):
   {TD_src = TD_tgt} + {TD_src <> TD_tgt}.
