coq/proof/SoundBase.v
@@ -1,0 +1,24 @@
+Require Import syntax.
+Require Import alist.
+Require Import FMapWeakList.
+
+Require Import Classical.
+Require Import Coqlib.
+Require Import infrastructure.
+Require Import Metatheory.
+Import LLVMsyntax.
+Import LLVMinfra.
+Require Import opsem.
+
+Require Import sflib.
+Require Import paco.
+Import Opsem.
+
+Require Import TODO.
+Require Import Validator.
+Require Import GenericValues.
+Require Import SimulationLocal.
+Require InvMem.
+Require InvState.
+
+Definition CONF_TODO: Prop. Admitted.
