coq/proof/SoundInfrules.v
@@ -1,0 +1,69 @@
+Require Import syntax.
+Require Import alist.
+Require Import FMapWeakList.
+
+Require Import Classical.
+Require Import Coqlib.
+Require Import infrastructure.
+Require Import Metatheory.
+Import LLVMsyntax.
+Import LLVMinfra.
+Require Import opsem.
+
+Require Import sflib.
+Require Import paco.
+Import Opsem.
+
+Require Import TODO.
+Require Import Validator.
+Require Import GenericValues.
+Require Import SimulationLocal.
+Require InvMem.
+Require InvState.
+Require Import SoundBase.
+
+Set Implicit Arguments.
+
+
+Lemma apply_infrule_sound
+      m_src m_tgt
+      conf_src st_src
+      conf_tgt st_tgt
+      invst0 invmem0 inv0
+      infrule
+      (CONF: CONF_TODO) (* m_src, m_tgt, conf_src, conf_tgt *)
+      (STATE: InvState.Rel.sem conf_src conf_tgt st_src st_tgt invst0 invmem0 inv0)
+      (MEM: InvMem.Rel.sem conf_src conf_tgt st_src.(Mem) st_tgt.(Mem) invmem0):
+  exists invst1 invmem1,
+    <<STATE: InvState.Rel.sem conf_src conf_tgt st_src st_tgt invst1 invmem1
+                              (Infrules.apply_infrule m_src m_tgt infrule inv0)>> /\
+    <<MEM: InvMem.Rel.sem conf_src conf_tgt st_src.(Mem) st_tgt.(Mem) invmem1>> /\
+    <<MEMLE: InvMem.Rel.le invmem0 invmem1>>.
+Proof.
+Admitted.
+
+Lemma apply_infrules_sound
+      m_src m_tgt
+      conf_src st_src
+      conf_tgt st_tgt
+      invst0 invmem0 inv0
+      infrules
+      (CONF: CONF_TODO) (* m_src, m_tgt, conf_src, conf_tgt *)
+      (STATE: InvState.Rel.sem conf_src conf_tgt st_src st_tgt invst0 invmem0 inv0)
+      (MEM: InvMem.Rel.sem conf_src conf_tgt st_src.(Mem) st_tgt.(Mem) invmem0):
+  exists invst1 invmem1,
+    <<STATE: InvState.Rel.sem conf_src conf_tgt st_src st_tgt invst1 invmem1
+                              (Infrules.apply_infrules m_src m_tgt infrules inv0)>> /\
+    <<MEM: InvMem.Rel.sem conf_src conf_tgt st_src.(Mem) st_tgt.(Mem) invmem1>> /\
+    <<MEMLE: InvMem.Rel.le invmem0 invmem1>>.
+Proof.
+  unfold Infrules.apply_infrules. rewrite <- fold_left_rev_right.
+  move infrules at top. revert_until infrules. induction (rev infrules); i.
+  - esplits; eauto.
+    admit. (* InvMem.Rel.le refl *)
+  - exploit IHl0; eauto. i. des.
+    exploit apply_infrule_sound; eauto. i. des.
+    esplits; eauto.
+    + ss. eauto.
+    + admit. (* InvMem.Rel.le trans *)
+Admitted.
