coq/proof/SoundPostcond.v
@@ -1,0 +1,53 @@
+Require Import syntax.
+Require Import alist.
+Require Import FMapWeakList.
+
+Require Import Classical.
+Require Import Coqlib.
+Require Import infrastructure.
+Require Import Metatheory.
+Import LLVMsyntax.
+Import LLVMinfra.
+Require Import opsem.
+
+Require Import sflib.
+Require Import paco.
+Import Opsem.
+
+Require Import TODO.
+Require Import Validator.
+Require Import GenericValues.
+Require Import SimulationLocal.
+Require InvMem.
+Require InvState.
+Require Import SoundBase.
+
+Set Implicit Arguments.
+
+
+Lemma has_false_False
+      conf_src conf_tgt st_src st_tgt invst invmem inv
+      (HAS_FALSE: Hints.Invariant.has_false inv)
+      (SEM: InvState.Rel.sem conf_src conf_tgt st_src st_tgt invst invmem inv):
+  False.
+Proof.
+Admitted.
+
+Lemma postcond_cmd_sound
+      conf_src st0_src cmd_src cmds_src
+      conf_tgt st0_tgt cmd_tgt cmds_tgt
+      invst0 invmem0 inv0
+      st1_tgt evt inv1
+      (CMDS_SRC: st0_src.(EC).(CurCmds) = cmd_src :: cmds_src)
+      (CMDS_TGT: st0_tgt.(EC).(CurCmds) = cmd_tgt :: cmds_tgt)
+      (POSTCOND: Postcond.postcond_cmd cmd_src cmd_tgt inv0 = Some inv1)
+      (STATE: InvState.Rel.sem conf_src conf_tgt st0_src st0_tgt invst0 invmem0 inv0)
+      (MEM: InvMem.Rel.sem conf_src conf_tgt st0_src.(Mem) st0_tgt.(Mem) invmem0)
+      (STEP_TGT: sInsn conf_tgt st0_tgt st1_tgt evt):
+  exists st1_src invst1 invmem1,
+    <<STEP_SRC: sInsn conf_src st0_src st1_src evt>> /\
+    <<STATE: InvState.Rel.sem conf_src conf_tgt st1_src st1_tgt invst1 invmem1 inv1>>/\
+    <<MEM: InvMem.Rel.sem conf_src conf_tgt st1_src.(Mem) st1_tgt.(Mem) invmem1>> /\
+    <<MEMLE: InvMem.Rel.le invmem0 invmem1>>.
+Proof.
+Admitted.
