coq/proof/SoundReduceMaydiff.v
@@ -1,0 +1,39 @@
+Require Import syntax.
+Require Import alist.
+Require Import FMapWeakList.
+
+Require Import Classical.
+Require Import Coqlib.
+Require Import infrastructure.
+Require Import Metatheory.
+Import LLVMsyntax.
+Import LLVMinfra.
+Require Import opsem.
+
+Require Import sflib.
+Require Import paco.
+Import Opsem.
+
+Require Import TODO.
+Require Import Validator.
+Require Import GenericValues.
+Require Import SimulationLocal.
+Require InvMem.
+Require InvState.
+Require Import SoundBase.
+
+Set Implicit Arguments.
+
+
+Lemma reduce_maydiff_sound
+      conf_src st_src
+      conf_tgt st_tgt
+      invst invmem inv
+      (CONF: CONF_TODO) (* m_src, m_tgt, conf_src, conf_tgt *)
+      (STATE: InvState.Rel.sem conf_src conf_tgt st_src st_tgt invst invmem inv)
+      (MEM: InvMem.Rel.sem conf_src conf_tgt st_src.(Mem) st_tgt.(Mem) invmem):
+  <<STATE: InvState.Rel.sem conf_src conf_tgt st_src st_tgt invst invmem
+                            (Postcond.reduce_maydiff inv)>> /\
+  <<MEM: InvMem.Rel.sem conf_src conf_tgt st_src.(Mem) st_tgt.(Mem) invmem>>.
+Proof.
+Admitted.
